cont.

Experiments/FSM_Impl.thy
@@ -35,6 +35,19 @@ fun fsm_impl_from_list :: "'a \<Rightarrow> ('a \<times> 'b \<times> 'c \<times>
                                       , outputs = image t_output ts'
                                       , transitions = ts' \<rparr>)"
 
+fun fsm_impl_from_list' :: "'a \<Rightarrow> ('a \<times> 'b \<times> 'c \<times> 'a) list \<Rightarrow> ('a, 'b, 'c) fsm_impl" where
+  "fsm_impl_from_list' q [] = \<lparr> initial = q, nodes = {q}, inputs = {}, outputs = {}, transitions = {} \<rparr>" |
+  "fsm_impl_from_list' q (t#ts) = (let tsr = (remdups (t#ts))
+                                   in \<lparr> initial = t_source t
+                                      , nodes = set (remdups ((map t_source tsr) @ (map t_target tsr)))
+                                      , inputs = set (remdups (map t_input tsr))
+                                      , outputs = set (remdups (map t_output tsr))
+                                      , transitions = set tsr \<rparr>)"
+
+lemma fsm_impl_from_list_code[code] :
+  "fsm_impl_from_list q ts = fsm_impl_from_list' q ts" 
+  by (cases ts; auto)
+
 subsection \<open>Changing the initial State\<close>
 
 fun from_FSM :: "('a,'b,'c) fsm_impl \<Rightarrow> 'a \<Rightarrow> ('a,'b,'c) fsm_impl" where
@@ -113,24 +126,30 @@ definition shifted_transitions :: "(('a \<times> 'a) \<times> 'b \<times> 'c \<t
   "shifted_transitions ts = image (\<lambda> t . (Inl (t_source t),t_input t, t_output t, Inl (t_target t))) ts"
 
 definition distinguishing_transitions :: "(('a \<times> 'b) \<Rightarrow> 'c set) \<Rightarrow> 'a \<Rightarrow> 'a \<Rightarrow> ('a \<times> 'a) set \<Rightarrow> 'b set \<Rightarrow> ((('a \<times> 'a) + 'a) \<times> 'b \<times> 'c \<times> (('a \<times> 'a) + 'a)) set" where
-  "distinguishing_transitions f q1 q2 nodeSet inputSet = \<Union> (Set.image (\<lambda>((q1',q2'),x) .  image (\<lambda>y . (Inl (q1',q2'),x,y,Inr q1)) (f (q1',x) - f (q2',x))) (nodeSet \<times> inputSet))"
+  "distinguishing_transitions f q1 q2 nodeSet inputSet = \<Union> (Set.image (\<lambda>((q1',q2'),x) .  
+                                                                (image (\<lambda>y . (Inl (q1',q2'),x,y,Inr q1)) (f (q1',x) - f (q2',x))) 
+                                                                \<union> (image (\<lambda>y . (Inl (q1',q2'),x,y,Inr q2)) (f (q2',x) - f (q1',x))))
+                                                            (nodeSet \<times> inputSet))"
 
 
-fun canonical_separator :: "('a,'b,'c) fsm_impl \<Rightarrow> (('a \<times> 'a),'b,'c) fsm_impl \<Rightarrow> 'a \<Rightarrow> 'a \<Rightarrow> (('a \<times> 'a) + 'a,'b,'c) fsm_impl" where
-  "canonical_separator M P q1 q2 = 
-  (let f'  = set_as_map (image (\<lambda>(q,x,y,q') . ((q,x),y)) (transitions M));
-       f   = (\<lambda>qx . (case f' qx of Some yqs \<Rightarrow> yqs | None \<Rightarrow> {}));
-       shifted_transitions' = shifted_transitions (transitions P);
-       distinguishing_transitions_left = distinguishing_transitions f q1 q2 (nodes P) (inputs P);
-       distinguishing_transitions_right = distinguishing_transitions f q2 q1 (nodes P) (inputs P);
-       ts = shifted_transitions' \<union> distinguishing_transitions_left \<union> distinguishing_transitions_right
-   in 
 
-    \<lparr> initial = Inl (q1,q2)
-    , nodes = insert (Inl (q1,q2)) ((image t_source ts) \<union> (image t_target ts))
-    , inputs = inputs M \<union> inputs P
-    , outputs = outputs M \<union> outputs P
-    , transitions = ts \<rparr>)"
+(* Note: parameter P is added to allow usage of different restricted versions of the product machine *)
+fun canonical_separator' :: "('a,'b,'c) fsm_impl \<Rightarrow> (('a \<times> 'a),'b,'c) fsm_impl \<Rightarrow> 'a \<Rightarrow> 'a \<Rightarrow> (('a \<times> 'a) + 'a,'b,'c) fsm_impl" where
+  "canonical_separator' M P q1 q2 = (if initial P = (q1,q2) 
+  then
+    (let f'  = set_as_map (image (\<lambda>(q,x,y,q') . ((q,x),y)) (transitions M));
+         f   = (\<lambda>qx . (case f' qx of Some yqs \<Rightarrow> yqs | None \<Rightarrow> {}));
+         shifted_transitions' = shifted_transitions (transitions P);
+         distinguishing_transitions_lr = distinguishing_transitions f q1 q2 (nodes P) (inputs P);
+         ts = shifted_transitions' \<union> distinguishing_transitions_lr
+     in 
+  
+      \<lparr> initial = Inl (q1,q2)
+      , nodes = (image Inl (nodes P)) \<union> {Inr q1, Inr q2}
+      , inputs = inputs M \<union> inputs P
+      , outputs = outputs M \<union> outputs P
+      , transitions = ts \<rparr>)
+  else \<lparr> initial = Inl (q1,q2), nodes = {Inl (q1,q2)}, inputs = {}, outputs = {}, transitions = {}\<rparr>)"
 
 
 
